LogicalRefinement/Wk.lean
@@ -3,11 +3,13 @@ inductive RawWk: Type 0 where
   | step: RawWk -> RawWk
   | lift: RawWk -> RawWk
 
-@[simp] def RawWk.wk1: RawWk := RawWk.step RawWk.id
+@[simp] def RawWk.wk1: RawWk := step id
 
 @[simp] def RawWk.liftn: (l: Nat) -> RawWk -> RawWk
   | 0, ρ => ρ
   | Nat.succ n, ρ => RawWk.lift (liftn n ρ)
+
+@[simp] def RawWk.wkn (n: Nat): RawWk := liftn n wk1
 
 @[simp] def RawWk.comp: RawWk -> RawWk -> RawWk
     | RawWk.id, σ => σ
